06/11/2015

float/fma_nonfma_llvm.c
@@ -1,0 +1,12 @@
+#pragma STDC FP_CONTRACT ON
+
+float f(float a, float b, float c){
+  float g = a * b + c;
+  return g;
+}
+
+int main(){
+  float a, b, c;
+  f(a, b, c);
+  return 0;
+}
