float/fma_nonfma_llvm.ll
@@ -1,0 +1,45 @@
+; ModuleID = 'fma_nonfma_llvm.c'
+target datalayout = "e-p:64:64:64-i1:8:8-i8:8:8-i16:16:16-i32:32:32-i64:64:64-f32:32:32-f64:64:64-v64:64:64-v128:128:128-a0:0:64-s0:64:64-f80:128:128-n8:16:32:64-S128"
+target triple = "x86_64-pc-linux-gnu"
+
+; Function Attrs: nounwind uwtable
+define float @f(float %a, float %b, float %c) #0 {
+  %1 = alloca float, align 4
+  %2 = alloca float, align 4
+  %3 = alloca float, align 4
+  %g = alloca float, align 4
+  store float %a, float* %1, align 4
+  store float %b, float* %2, align 4
+  store float %c, float* %3, align 4
+  %4 = load float* %1, align 4
+  %5 = load float* %2, align 4
+  %6 = load float* %3, align 4
+  %7 = call float @llvm.fmuladd.f32(float %4, float %5, float %6)
+  store float %7, float* %g, align 4
+  %8 = load float* %g, align 4
+  ret float %8
+}
+
+; Function Attrs: nounwind readnone
+declare float @llvm.fmuladd.f32(float, float, float) #1
+
+; Function Attrs: nounwind uwtable
+define i32 @main() #0 {
+  %1 = alloca i32, align 4
+  %a = alloca float, align 4
+  %b = alloca float, align 4
+  %c = alloca float, align 4
+  store i32 0, i32* %1
+  %2 = load float* %a, align 4
+  %3 = load float* %b, align 4
+  %4 = load float* %c, align 4
+  %5 = call float @f(float %2, float %3, float %4)
+  ret i32 0
+}
+
+attributes #0 = { nounwind uwtable "less-precise-fpmad"="false" "no-frame-pointer-elim"="true" "no-frame-pointer-elim-non-leaf" "no-infs-fp-math"="false" "no-nans-fp-math"="false" "stack-protector-buffer-size"="8" "unsafe-fp-math"="false" "use-soft-float"="false" }
+attributes #1 = { nounwind readnone }
+
+!llvm.ident = !{!0}
+
+!0 = metadata !{metadata !"Ubuntu clang version 3.4.2- (branches/release_34) (based on LLVM 3.4.2)"}
